Bignum/ArmRev/InstructionLemmas.lean
@@ -16,4 +16,13 @@ namespace Bignum.ArmRev.State
 theorem XZR_zero : XZR = Component.rvalue 0 := by
   rfl
 
+theorem WZR_zero : WZR = Component.rvalue 0 := by
+  rfl
+
+theorem ZR_zero (w : Nat) : @ZR w = Component.rvalue 0 := by
+  rfl
+
+theorem XREG31_zero : XREG 31 = Component.rvalue 0 := by
+  rfl
+
 end Bignum.ArmRev.State
